OeufProof done down through Fmajor

src/Oeuf.v
@@ -14,29 +14,98 @@ Require compcert.backend.SelectLong.
 Require Import Linker.
 
 
-Definition transf_untyped_to_cminor (l : list Untyped1.expr * list Metadata.metadata) : res Cminor.program :=
+Definition transf_untyped_to_tagged (l : list Untyped1.expr * list Metadata.metadata) :=
   OK l
  @@@ UntypedCompCombined.compile_cu
- @@@ TaggedComp.compile_cu ~~ "TaggedComp"
-  @@ TaggedNumberedComp.compile_cu
- @@@ ElimFuncComp.compile_cu
- @@@ ElimFuncComp2.compile_cu ~~ "ElimFuncComp2"
- @@@ ElimFuncComp3.compile_cu ~~ "ElimFuncComp3"
- @@@ SwitchedComp.compile_cu ~~ "SwitchedComp"
-  @@ SelfCloseComp.compile_cu
-  @@ ValueFlagComp.compile_cu
- @@@ StackCompCombined.compile_cu
- @@@ LocalsCompCombined.compile_cu
- @@@ FlatCompCombined.compile_cu
- @@@ FmajorComp.compile_cu ~~ "FmajorComp"
-  @@ Fmajortofflatmajor.transf_program
-  @@ Fflatmajortoemajor.transf_program
-  @@@ Emajortodmajor.transf_prog
-  @@@ Dmajortodflatmajor.transf_prog
- @@@ Dflatmajortocmajor.transf_prog
+ @@@ TaggedComp.compile_cu ~~ "TaggedComp".
+
+Definition transf_untyped_to_tagged_numbered (l : list Untyped1.expr * list Metadata.metadata)  :=
+  OK l
+  @@@ transf_untyped_to_tagged
+  @@ TaggedNumberedComp.compile_cu.
+
+Definition transf_untyped_to_elim_func (l : list Untyped1.expr * list Metadata.metadata)  :=
+  OK l
+  @@@ transf_untyped_to_tagged_numbered
+  @@@ ElimFuncComp.compile_cu.
+ 
+Definition transf_untyped_to_elim_func2 (l : list Untyped1.expr * list Metadata.metadata)  :=
+  OK l
+  @@@ transf_untyped_to_elim_func
+  @@@ ElimFuncComp2.compile_cu.
+
+Definition transf_untyped_to_elim_func3 (l : list Untyped1.expr * list Metadata.metadata)  :=
+  OK l
+  @@@ transf_untyped_to_elim_func2
+  @@@ ElimFuncComp3.compile_cu.
+
+Definition transf_untyped_to_switched (l : list Untyped1.expr * list Metadata.metadata)  :=
+  OK l
+  @@@ transf_untyped_to_elim_func3
+  @@@ SwitchedComp.compile_cu ~~ "SwitchedComp".
+
+Definition transf_untyped_to_self_close (l : list Untyped1.expr * list Metadata.metadata)  :=
+  OK l
+  @@@ transf_untyped_to_switched
+  @@ SelfCloseComp.compile_cu.
+
+Definition transf_untyped_to_value_flag (l : list Untyped1.expr * list Metadata.metadata)  :=
+  OK l
+  @@@ transf_untyped_to_self_close
+  @@ ValueFlagComp.compile_cu.
+
+Definition transf_untyped_to_stack (l : list Untyped1.expr * list Metadata.metadata)  :=
+  OK l
+  @@@ transf_untyped_to_value_flag
+  @@@ StackCompCombined.compile_cu.
+
+Definition transf_untyped_to_locals (l : list Untyped1.expr * list Metadata.metadata)  :=
+  OK l
+  @@@ transf_untyped_to_stack
+  @@@ LocalsCompCombined.compile_cu.
+
+Definition transf_untyped_to_flat (l : list Untyped1.expr * list Metadata.metadata)  :=
+  OK l
+  @@@ transf_untyped_to_locals
+  @@@ FlatCompCombined.compile_cu.
+
+Definition transf_untyped_to_fmajor (l : list Untyped1.expr * list Metadata.metadata)  :=
+  OK l
+  @@@ transf_untyped_to_flat
+  @@@ FmajorComp.compile_cu ~~ "FmajorComp".
+
+Definition transf_untyped_to_fflatmajor (l : list Untyped1.expr * list Metadata.metadata)  :=
+  OK l
+  @@@ transf_untyped_to_fmajor
+  @@ Fmajortofflatmajor.transf_program.
+
+Definition transf_untyped_to_emajor (l : list Untyped1.expr * list Metadata.metadata)  :=
+  OK l
+  @@@ transf_untyped_to_fflatmajor
+  @@ Fflatmajortoemajor.transf_program.
+
+Definition transf_untyped_to_dmajor (l : list Untyped1.expr * list Metadata.metadata)  :=
+  OK l
+  @@@ transf_untyped_to_emajor
+  @@@ Emajortodmajor.transf_prog.
+
+Definition transf_untyped_to_dflatmajor (l : list Untyped1.expr * list Metadata.metadata)  :=
+  OK l
+  @@@ transf_untyped_to_dmajor
+  @@@ Dmajortodflatmajor.transf_prog.
+
+Definition transf_untyped_to_cmajor (l : list Untyped1.expr * list Metadata.metadata)  :=
+  OK l
+  @@@ transf_untyped_to_dflatmajor
+  @@@ Dflatmajortocmajor.transf_prog.
+
+
+Definition transf_untyped_to_cminor (l : list Untyped1.expr * list Metadata.metadata) : res Cminor.program :=
+  OK l
+  @@@ transf_untyped_to_cmajor
   @@ Cmajortominor.transf_prog
-  @@ print print_Cminor
-.
+  @@ print print_Cminor.
+
 
 Definition transf_oeuf_to_untyped1 (j : CompilationUnit.compilation_unit) : res Untyped1.prog_type :=
   OK (Metadata.init_metadata j)
@@ -73,7 +142,8 @@ Definition transf_whole_program (oeuf_code : CompilationUnit.compilation_unit) (
   | Error m => Error m
   end.
                                     
-(* LEGACY BELOW *)  
+(* LEGACY BELOW *)
+(*
 Definition transf_to_cminor (j : CompilationUnit.compilation_unit) : res Cminor.program :=
   OK (Metadata.init_metadata j)
   @@ UntypedComp1.compile_cu
@@ -84,4 +154,4 @@ Definition transf_to_cminor (j : CompilationUnit.compilation_unit) : res Cminor.
 Definition transf_to_asm (j : CompilationUnit.compilation_unit) : res Asm.program :=
   transf_to_cminor j
  @@@ transf_cminor_program.
-
+*)
